src/3d/Batch.fsti
@@ -4,6 +4,7 @@ open FStar.All
 val postprocess
   (clang_format: bool)
   (clang_format_executable: string)
+  (cleanup: bool)
   (out_dir: string)
   (files_and_modules: list (string & string))
 : ML unit
