src/3d/Main.fst
@@ -84,7 +84,12 @@ let go () : ML unit =
   let out_dir = Options.get_output_dir () in
   let files_and_modules = List.map (fun file -> (file, Options.get_module_name file)) files in
   if Options.get_batch ()
-  then Batch.postprocess (Options.get_clang_format ()) (Options.get_clang_format_executable ()) out_dir files_and_modules;
+  then
+    Batch.postprocess
+      (Options.get_clang_format ())
+      (Options.get_clang_format_executable ())
+      (Options.get_cleanup ())
+      out_dir files_and_modules;
   FStar.IO.print_string "EverParse succeeded!\n"
 
 #push-options "--warn_error -272" //top-level effects are okay
